aarch64/Asm.v
@@ -307,7 +307,7 @@ Inductive instruction: Type :=
 .
 
 Definition code := list instruction.
-Record function : Type := mkfunction { fn_sig: signature; fn_code: code }.
+Record function : Type := mkfunction { fn_sig: signature; fn_code: code; fn_stacksize : Z }.
 Definition fundef := AST.fundef function.
 Definition program := AST.program fundef unit.
 
@@ -1065,9 +1065,13 @@ Definition exec_instr (f: function) (i: instruction) (rs: regset) (m: mem) : out
   | Pallocframe sz pos =>
       let (m1, stk) := Mem.alloc m 0 sz in
       let sp := (Vptr stk Ptrofs.zero) in
-      match Mem.storev Mint64 m1 (Val.offset_ptr sp pos) rs#SP with
-      | None => Stuck
-      | Some m2 => Next (nextinstr (rs #X29 <- (rs#SP) #SP <- sp #X16 <- Vundef)) m2
+      match Mem.record_frame (Mem.push_stage m1) (Mem.mk_frame sz) with
+        |None => Stuck
+        |Some m2 =>
+         match Mem.storev Mint64 m2 (Val.offset_ptr sp pos) rs#SP with
+         | None => Stuck
+         | Some m3 => Next (nextinstr (rs #X29 <- (rs#SP) #SP <- sp #X16 <- Vundef)) m3
+         end
       end
   | Pfreeframe sz pos =>
       match Mem.loadv Mint64 m (Val.offset_ptr rs#SP pos) with
@@ -1077,7 +1081,11 @@ Definition exec_instr (f: function) (i: instruction) (rs: regset) (m: mem) : out
           | Vptr stk ofs =>
               match Mem.free m stk 0 sz with
               | None => Stuck
-              | Some m' => Next (nextinstr (rs#SP <- v #X16 <- Vundef)) m'
+              | Some m' =>
+                match Mem.pop_stage m'  with
+                  |None => Stuck
+                  |Some m'' => Next (nextinstr (rs#SP <- v #X16 <- Vundef)) m''
+                end
               end
           | _ => Stuck
           end
