riscV/Asm.v
@@ -426,7 +426,7 @@ table:  .long   table[0], table[1], ...
 *)
 
 Definition code := list instruction.
-Record function : Type := mkfunction { fn_sig: signature; fn_code: code }.
+Record function : Type := mkfunction { fn_sig: signature; fn_code: code; fn_stacksize : Z }.
 Definition fundef := AST.fundef function.
 Definition program := AST.program fundef unit.
 
@@ -925,9 +925,13 @@ Definition exec_instr (f: function) (i: instruction) (rs: regset) (m: mem) : out
   | Pallocframe sz pos =>
       let (m1, stk) := Mem.alloc m 0 sz in
       let sp := (Vptr stk Ptrofs.zero) in
-      match Mem.storev Mptr m1 (Val.offset_ptr sp pos) rs#SP with
-      | None => Stuck
-      | Some m2 => Next (nextinstr (rs #X30 <- (rs SP) #SP <- sp #X31 <- Vundef)) m2
+      match Mem.record_frame (Mem.push_stage m1) (Mem.mk_frame sz) with
+        |None => Stuck
+        |Some m2 =>
+         match Mem.storev Mptr m2 (Val.offset_ptr sp pos) rs#SP with
+         | None => Stuck
+         | Some m3 => Next (nextinstr (rs #X30 <- (rs SP) #SP <- sp #X31 <- Vundef)) m3
+         end
       end
   | Pfreeframe sz pos =>
       match Mem.loadv Mptr m (Val.offset_ptr rs#SP pos) with
@@ -937,7 +941,11 @@ Definition exec_instr (f: function) (i: instruction) (rs: regset) (m: mem) : out
           | Vptr stk ofs =>
               match Mem.free m stk 0 sz with
               | None => Stuck
-              | Some m' => Next (nextinstr (rs#SP <- v #X31 <- Vundef)) m'
+              | Some m' =>
+                match Mem.pop_stage m' with
+                  |None => Stuck
+                  |Some m'' => Next (nextinstr (rs#SP <- v #X31 <- Vundef)) m''
+                end
               end
           | _ => Stuck
           end
