aarch64/Asmgenproof1.v
@@ -1794,42 +1794,44 @@ Proof.
 Qed.
 
 Lemma make_epilogue_correct:
-  forall ge0 f m stk soff cs m' ms rs k tm,
+  forall ge0 f m stk soff cs m' m'' ms rs k tm,
   load_stack m (Vptr stk soff) Tptr f.(fn_link_ofs) = Some (parent_sp cs) ->
   load_stack m (Vptr stk soff) Tptr f.(fn_retaddr_ofs) = Some (parent_ra cs) ->
-  Mem.free m stk 0 f.(fn_stacksize) = Some m' ->
+  Mem.free m stk 0 f.(Mach.fn_stacksize) = Some m' ->
+  Mem.pop_stage m' = Some m'' ->
   agree ms (Vptr stk soff) rs ->
   Mem.extends m tm ->
   match_stack ge0 cs ->
-  exists rs', exists tm',
-     exec_straight ge fn (make_epilogue f k) rs tm k rs' tm'
+  exists rs', exists tm'',
+     exec_straight ge fn (make_epilogue f k) rs tm k rs' tm''
   /\ agree ms (parent_sp cs) rs'
-  /\ Mem.extends m' tm'
+  /\ Mem.extends m'' tm''
   /\ rs'#RA = parent_ra cs
   /\ rs'#SP = parent_sp cs
   /\ (forall r, r <> PC -> r <> SP -> r <> X30 -> r <> X16 -> rs'#r = rs#r).
 Proof.
-  intros until tm; intros LP LRA FREE AG MEXT MCS.
+  intros until tm; intros LP LRA FREE POP AG MEXT MCS.
   exploit Mem.loadv_extends. eauto. eexact LP. auto. simpl. intros (parent' & LP' & LDP').
   exploit Mem.loadv_extends. eauto. eexact LRA. auto. simpl. intros (ra' & LRA' & LDRA').
   exploit lessdef_parent_sp; eauto. intros EQ; subst parent'; clear LDP'.
   exploit lessdef_parent_ra; eauto. intros EQ; subst ra'; clear LDRA'.
   exploit Mem.free_parallel_extends; eauto. intros (tm' & FREE' & MEXT').
-  unfold make_epilogue. 
+  exploit Mem.pop_stage_extends; eauto. intros (tm'' & POP' & MEXT'' ).
+  unfold make_epilogue.
   exploit (loadptr_correct XSP (fn_retaddr_ofs f)).
     instantiate (2 := rs). simpl. rewrite <- (sp_val _ _ _ AG). simpl. eexact LRA'. simpl; congruence.
   intros (rs1 & A1 & B1 & C1).
   econstructor; econstructor; split.
-  eapply exec_straight_trans. eexact A1. apply exec_straight_one. simpl. 
-    simpl; rewrite (C1 SP) by auto with asmgen. rewrite <- (sp_val _ _ _ AG). simpl; rewrite LP'. 
-    rewrite FREE'. eauto. auto. 
+  eapply exec_straight_trans. eexact A1. apply exec_straight_one. simpl.
+    simpl; rewrite (C1 SP) by auto with asmgen. rewrite <- (sp_val _ _ _ AG). simpl; rewrite LP'.
+    rewrite FREE'. rewrite POP'. eauto. auto.
   split. apply agree_nextinstr. apply agree_set_other; auto.
   apply agree_change_sp with (Vptr stk soff).
   apply agree_exten with rs; auto. intros; apply C1; auto with asmgen.
   eapply parent_sp_def; eauto.
   split. auto.
-  split. Simpl. 
-  split. Simpl. 
+  split. Simpl.
+  split. Simpl.
   intros. Simpl.
 Qed.
 
