riscV/Asmgenproof.v
@@ -700,12 +700,12 @@ Opaque loadind.
 - (* Mop *)
   assert (eval_operation tge sp op (map rs args) m = Some v).
     rewrite <- H. apply eval_operation_preserved. exact symbols_preserved.
-  exploit eval_operation_lessdef. eapply preg_vals; eauto. eauto. eexact H0.
+  exploit eval_operation_lessdef. eapply preg_vals; eauto. apply MEXT. eexact H0.
   intros [v' [A B]]. rewrite (sp_val _ _ _ AG) in A.
   left; eapply exec_straight_steps; eauto; intros. simpl in TR.
   exploit transl_op_correct; eauto. intros [rs2 [P [Q R]]].
   exists rs2; split. eauto. split. auto.
-  apply agree_set_undef_mreg with rs0; auto. 
+  apply agree_set_undef_mreg with rs0; auto.
   apply Val.lessdef_trans with v'; auto.
   simpl; intros. destruct (andb_prop _ _ H1); clear H1.
   rewrite R; auto. apply preg_of_not_X30; auto.
@@ -743,28 +743,28 @@ Local Transparent destroyed_by_op.
   inv AT.
   assert (NOOV: list_length_z tf.(fn_code) <= Ptrofs.max_unsigned).
     eapply transf_function_no_overflow; eauto.
-  destruct ros as [rf|fid]; simpl in H; monadInv H5.
+  destruct ros as [rf|fid]; simpl in H; monadInv H6.
 + (* Indirect call *)
   assert (rs rf = Vptr f' Ptrofs.zero).
     destruct (rs rf); try discriminate.
     revert H; predSpec Ptrofs.eq Ptrofs.eq_spec i Ptrofs.zero; intros; congruence.
   assert (rs0 x0 = Vptr f' Ptrofs.zero).
-    exploit ireg_val; eauto. rewrite H5; intros LD; inv LD; auto.
-  generalize (code_tail_next_int _ _ _ _ NOOV H6). intro CT1.
+    exploit ireg_val; eauto. rewrite H6; intros LD; inv LD; auto.
+  generalize (code_tail_next_int _ _ _ _ NOOV H7). intro CT1.
   assert (TCA: transl_code_at_pc ge (Vptr fb (Ptrofs.add ofs Ptrofs.one)) fb f c false tf x).
     econstructor; eauto.
   exploit return_address_offset_correct; eauto. intros; subst ra.
   left; econstructor; split.
-  apply plus_one. eapply exec_step_internal. Simpl. rewrite <- H2; simpl; eauto.
+  apply plus_one. eapply exec_step_internal. Simpl. rewrite <- H3; simpl; eauto.
   eapply functions_transl; eauto. eapply find_instr_tail; eauto.
   simpl. eauto.
   econstructor; eauto.
   econstructor; eauto.
   eapply agree_sp_def; eauto.
   simpl. eapply agree_exten; eauto. intros. Simpl.
-  Simpl. rewrite <- H2. auto.
+  Simpl. rewrite <- H3. auto.
 + (* Direct call *)
-  generalize (code_tail_next_int _ _ _ _ NOOV H6). intro CT1.
+  generalize (code_tail_next_int _ _ _ _ NOOV H7). intro CT1.
   assert (TCA: transl_code_at_pc ge (Vptr fb (Ptrofs.add ofs Ptrofs.one)) fb f c false tf x).
     econstructor; eauto.
   exploit return_address_offset_correct; eauto. intros; subst ra.
@@ -776,22 +776,22 @@ Local Transparent destroyed_by_op.
   econstructor; eauto.
   eapply agree_sp_def; eauto.
   simpl. eapply agree_exten; eauto. intros. Simpl.
-  Simpl. rewrite <- H2. auto.
+  Simpl. rewrite <- H3. auto.
 
 - (* Mtailcall *)
   assert (f0 = f) by congruence.  subst f0.
   inversion AT; subst.
   assert (NOOV: list_length_z tf.(fn_code) <= Ptrofs.max_unsigned).
-    eapply transf_function_no_overflow; eauto.  exploit Mem.loadv_extends. eauto. eexact H1. auto. simpl. intros [parent' [A B]].
-  destruct ros as [rf|fid]; simpl in H; monadInv H7.
+    eapply transf_function_no_overflow; eauto.  exploit Mem.loadv_extends. eauto. eexact H2. auto. simpl. intros [parent' [A B]].
+  destruct ros as [rf|fid]; simpl in H; monadInv H9.
 + (* Indirect call *)
   assert (rs rf = Vptr f' Ptrofs.zero).
     destruct (rs rf); try discriminate.
     revert H; predSpec Ptrofs.eq Ptrofs.eq_spec i Ptrofs.zero; intros; congruence.
   assert (rs0 x0 = Vptr f' Ptrofs.zero).
-    exploit ireg_val; eauto. rewrite H7; intros LD; inv LD; auto.
-  exploit make_epilogue_correct; eauto. intros (rs1 & m1 & U & V & W & X & Y & Z). 
-  exploit exec_straight_steps_2; eauto using functions_transl.                      
+    exploit ireg_val; eauto. rewrite H9; intros LD; inv LD; auto.
+  exploit make_epilogue_correct; eauto. intros (rs1 & m1 & U & V & W & X & Y & Z).
+  exploit exec_straight_steps_2; eauto using functions_transl.
   intros (ofs' & P & Q).
   left; econstructor; split.
   (* execution *)
@@ -802,10 +802,10 @@ Local Transparent destroyed_by_op.
   (* match states *)
   econstructor; eauto.
   apply agree_set_other; auto with asmgen.
-  Simpl. rewrite Z by (rewrite <- (ireg_of_eq _ _ EQ1); eauto with asmgen). assumption. 
+  Simpl. rewrite Z by (rewrite <- (ireg_of_eq _ _ EQ1); eauto with asmgen). assumption.
 + (* Direct call *)
-  exploit make_epilogue_correct; eauto. intros (rs1 & m1 & U & V & W & X & Y & Z). 
-  exploit exec_straight_steps_2; eauto using functions_transl.                      
+  exploit make_epilogue_correct; eauto. intros (rs1 & m1 & U & V & W & X & Y & Z).
+  exploit exec_straight_steps_2; eauto using functions_transl.
   intros (ofs' & P & Q).
   left; econstructor; split.
   (* execution *)
@@ -835,7 +835,7 @@ Local Transparent destroyed_by_op.
   econstructor; eauto.
   instantiate (2 := tf); instantiate (1 := x).
   unfold nextinstr. rewrite Pregmap.gss.
-  rewrite set_res_other. rewrite undef_regs_other_2. rewrite Pregmap.gso by congruence. 
+  rewrite set_res_other. rewrite undef_regs_other_2. rewrite Pregmap.gso by congruence.
   rewrite <- H1. simpl. econstructor; eauto.
   eapply code_tail_next_int; eauto.
   rewrite preg_notin_charact. intros. auto with asmgen.
@@ -859,17 +859,17 @@ Local Transparent destroyed_by_op.
 
 - (* Mcond true *)
   assert (f0 = f) by congruence. subst f0.
-  exploit eval_condition_lessdef. eapply preg_vals; eauto. eauto. eauto. intros EC.
+  exploit eval_condition_lessdef. eapply preg_vals; eauto. apply MEXT. eauto. intros EC.
   left; eapply exec_straight_opt_steps_goto; eauto.
   intros. simpl in TR.
   exploit transl_cbranch_correct_true; eauto. intros (rs' & jmp & A & B & C).
   exists jmp; exists k; exists rs'.
-  split. eexact A. 
+  split. eexact A.
   split. apply agree_exten with rs0; auto with asmgen.
-  exact B. 
+  exact B.
 
 - (* Mcond false *)
-  exploit eval_condition_lessdef. eapply preg_vals; eauto. eauto. eauto. intros EC.
+  exploit eval_condition_lessdef. eapply preg_vals; eauto. apply MEXT. eauto. intros EC.
   left; eapply exec_straight_steps; eauto. intros. simpl in TR.
   exploit transl_cbranch_correct_false; eauto. intros (rs' & A & B).
   exists rs'.
@@ -899,11 +899,11 @@ Local Transparent destroyed_by_op.
 
 - (* Mreturn *)
   assert (f0 = f) by congruence. subst f0.
-  inversion AT; subst. simpl in H6; monadInv H6.
+  inversion AT; subst. simpl in H7; monadInv H7.
   assert (NOOV: list_length_z tf.(fn_code) <= Ptrofs.max_unsigned).
     eapply transf_function_no_overflow; eauto.
   exploit make_epilogue_correct; eauto. intros (rs1 & m1 & U & V & W & X & Y & Z).
-  exploit exec_straight_steps_2; eauto using functions_transl.                      
+  exploit exec_straight_steps_2; eauto using functions_transl.
   intros (ofs' & P & Q).
   left; econstructor; split.
   (* execution *)
@@ -922,42 +922,45 @@ Local Transparent destroyed_by_op.
   unfold store_stack in *.
   exploit Mem.alloc_extends. eauto. eauto. apply Z.le_refl. apply Z.le_refl.
   intros [m1' [C D]].
-  exploit Mem.storev_extends. eexact D. eexact H1. eauto. eauto.
-  intros [m2' [F G]].
+  exploit Mem.push_stage_extends; eauto. intro.
+  exploit Mem.record_frame_extends; eauto.
+  intros [m2' [E F]].
+  exploit Mem.storev_extends. eexact F. eexact H2. eauto. eauto.
+  intros [m3' [G O]].
   simpl chunk_of_type in F.
-  exploit Mem.storev_extends. eexact G. eexact H2. eauto. eauto.
-  intros [m3' [P Q]].
+  exploit Mem.storev_extends. eexact O. eexact H3. eauto. eauto.
+  intros [m4' [P Q]].
   (* Execution of function prologue *)
   monadInv EQ0. rewrite transl_code'_transl_code in EQ1.
-  set (tfbody := Pallocframe (fn_stacksize f) (fn_link_ofs f) ::
+  set (tfbody := Pallocframe (Mach.fn_stacksize f) (fn_link_ofs f) ::
                  storeind_ptr RA SP (fn_retaddr_ofs f) x0) in *.
-  set (tf := {| fn_sig := Mach.fn_sig f; fn_code := tfbody |}) in *.
+  set (tf := {| fn_sig := Mach.fn_sig f; fn_code := tfbody; fn_stacksize := Mach.fn_stacksize f |}) in *.
   set (rs2 := nextinstr (rs0#X30 <- (parent_sp s) #SP <- sp #X31 <- Vundef)).
-  exploit (storeind_ptr_correct tge tf SP (fn_retaddr_ofs f) RA x0 rs2 m2').
-    rewrite chunk_of_Tptr in P. change (rs2 X1) with (rs0 X1). rewrite ATLR. 
-    change (rs2 X2) with sp. eexact P. 
+  exploit (storeind_ptr_correct tge tf SP (fn_retaddr_ofs f) RA x0 rs2 m3').
+    rewrite chunk_of_Tptr in P. change (rs2 X1) with (rs0 X1). rewrite ATLR.
+    change (rs2 X2) with sp. eexact P.
     congruence. congruence.
   intros (rs3 & U & V).
   assert (EXEC_PROLOGUE:
             exec_straight tge tf
               tf.(fn_code) rs0 m'
-              x0 rs3 m3').
+              x0 rs3 m4').
   { change (fn_code tf) with tfbody; unfold tfbody.
-    apply exec_straight_step with rs2 m2'.
-    unfold exec_instr. rewrite C. fold sp.
-    rewrite <- (sp_val _ _ _ AG). rewrite chunk_of_Tptr in F. rewrite F. reflexivity.
-    reflexivity. 
+    apply exec_straight_step with rs2 m3'.
+    unfold exec_instr. rewrite C. rewrite E. fold sp.
+    rewrite <- (sp_val _ _ _ AG). rewrite chunk_of_Tptr in G. rewrite G. reflexivity.
+    reflexivity.
     eexact U. }
   exploit exec_straight_steps_2; eauto using functions_transl. lia. constructor.
-  intros (ofs' & X & Y).                    
-  left; exists (State rs3 m3'); split.
+  intros (ofs' & X & Y).
+  left; exists (State rs3 m4'); split.
   eapply exec_straight_steps_1; eauto. lia. constructor.
   econstructor; eauto.
-  rewrite X; econstructor; eauto. 
+  rewrite X; econstructor; eauto.
   apply agree_exten with rs2; eauto with asmgen.
-  unfold rs2. 
+  unfold rs2.
   apply agree_nextinstr. apply agree_set_other; auto with asmgen.
-  apply agree_change_sp with (parent_sp s). 
+  apply agree_change_sp with (parent_sp s).
   apply agree_undef_regs with rs0. auto.
 Local Transparent destroyed_at_function_entry.
   simpl; intros; Simpl.
@@ -976,7 +979,7 @@ Local Transparent destroyed_at_function_entry.
   eapply external_call_symbols_preserved; eauto. apply senv_preserved.
   econstructor; eauto.
   unfold loc_external_result. apply agree_set_other; auto. apply agree_set_pair; auto.
-  apply agree_undef_caller_save_regs; auto. 
+  apply agree_undef_caller_save_regs; auto.
 
 - (* return *)
   inv STACKS. simpl in *.
